riscv access: add proofs for Syscall_AC
Signed-off-by: Ryan Barry <ryan.barry@unsw.edu.au>

proof/access-control/Syscall_AC.thy
@@ -32,14 +32,14 @@ definition authorised_invocation ::
                                                      \<and> cnode_inv_auth_derivations i' s
    | InvokeIRQControl i' \<Rightarrow> authorised_irq_ctl_inv aag i'
    | InvokeIRQHandler i' \<Rightarrow> authorised_irq_hdl_inv aag i'
-   | InvokeArchObject i' \<Rightarrow> valid_arch_inv i' s \<and> authorised_arch_inv aag i' \<and> ct_active s"
+   | InvokeArchObject i' \<Rightarrow> valid_arch_inv i' s \<and> authorised_arch_inv aag i' s \<and> ct_active s"
 
 lemma perform_invocation_pas_refined:
   "\<lbrace>pas_refined aag and pas_cur_domain aag and einvs and simple_sched_action
                     and valid_invocation oper and is_subject aag \<circ> cur_thread
                     and authorised_invocation aag oper\<rbrace>
    perform_invocation blocking calling oper
-   \<lbrace>\<lambda>rv. pas_refined aag\<rbrace>"
+   \<lbrace>\<lambda>_. pas_refined aag\<rbrace>"
   apply (cases oper, simp_all)
            apply (simp add: authorised_invocation_def validE_R_def[symmetric] invs_valid_objs
                   | wp invoke_untyped_pas_refined send_ipc_pas_refined send_signal_pas_refined
@@ -105,12 +105,13 @@ lemma perform_invocation_respects:
 
 declare AllowSend_def[simp] AllowRecv_def[simp]
 
-(* FIXME AC: breaks for RISCV unless "real_cte_at slot" is assumed. This term appears in the RISCV
-             variant of arch_decode_inv_wf, but not in the ARM variant. We should avoid requalifying
-             it and instead have a wp rule for valid_arch_inv as part of a locale. *)
+(* FIXME AC: the RISCV variant of arch_decode_inv_wf assumes "real_cte_at slot" whereas the
+             ARM variant does not. Just going to assume "real_cte_at slot" here for now even
+             though it's redundant for ARM. *)
 lemma decode_invocation_authorised:
   "\<lbrace>pas_refined aag and valid_cap cap and invs and ct_active and (is_subject aag \<circ> cur_thread) and
     cte_wp_at ((=) cap) slot and ex_cte_cap_to slot and domain_sep_inv (pasMaySendIrqs aag) st' and
+    real_cte_at slot and
     (\<lambda>s. \<forall>r\<in>zobj_refs cap. ex_nonz_cap_to r s) and
     (\<lambda>s. \<forall>r\<in>cte_refs cap (interrupt_irq_node s). ex_cte_cap_to r s) and
     (\<lambda>s. \<forall>cap \<in> set excaps. \<forall>r\<in>cte_refs (fst cap) (interrupt_irq_node s). ex_cte_cap_to r s) and
@@ -136,7 +137,6 @@ lemma decode_invocation_authorised:
           | wpc | simp add: comp_def authorised_invocation_def decode_invocation_def
                        split del: if_split del: hoare_True_E_R
           | wp (once) hoare_FalseE_R)+
-
   apply (clarsimp simp: aag_has_Control_iff_owns split_def aag_cap_auth_def)
   apply (cases cap, simp_all)
           apply (fastforce simp: cte_wp_at_caps_of_state)
@@ -159,10 +159,8 @@ lemma decode_invocation_authorised:
      apply (simp only: domain_sep_inv_def)
     apply (rule impI, erule subst, rule pas_refined_sita_mem [OF sita_controlled],
            auto simp: cte_wp_at_caps_of_state)[1]
-
    apply (clarsimp simp add: cap_links_irq_def )
    apply (drule (1) pas_refined_Control, simp)
-
   apply (clarsimp simp: cap_links_asid_slot_def label_owns_asid_slot_def)
   apply (fastforce dest!: pas_refined_Control)
   done
@@ -171,10 +169,15 @@ lemma in_extended: "(u,a) \<in> fst (do_extended_op f s) \<Longrightarrow> \<exi
   by (fastforce simp: do_extended_op_def bind_def gets_def return_def get_def
                       mk_ef_def modify_def select_f_def put_def trans_state_update')
 
+lemma set_scheduler_action_authorised_arch_inv[wp]:
+  "set_scheduler_action act \<lbrace>authorised_arch_inv aag i\<rbrace>"
+  unfolding set_scheduler_action_def
+  by wpsimp
+
 lemma set_thread_state_authorised[wp]:
   "\<lbrace>authorised_invocation aag i and (\<lambda>s. thread = cur_thread s) and valid_objs\<rbrace>
    set_thread_state thread Restart
-   \<lbrace>\<lambda>rv. authorised_invocation aag i\<rbrace>"
+   \<lbrace>\<lambda>_. authorised_invocation aag i\<rbrace>"
   apply (cases i; simp add: authorised_invocation_def)
           apply (wpsimp wp: sts_valid_untyped_inv ct_in_state_set
                             hoare_vcg_ex_lift sts_obj_at_impossible)+
@@ -188,7 +191,7 @@ lemma set_thread_state_authorised[wp]:
 
 lemma sts_first_restart:
   "\<lbrace>(=) st and (\<lambda>s. thread = cur_thread s)\<rbrace>
-     set_thread_state thread Structures_A.thread_state.Restart
+   set_thread_state thread Structures_A.thread_state.Restart
    \<lbrace>\<lambda>rv s. \<forall>p ko. kheap s p = Some ko \<longrightarrow>
            (is_tcb ko \<longrightarrow> p \<noteq> cur_thread st) \<longrightarrow> kheap st p = Some ko\<rbrace>"
   unfolding set_thread_state_def
@@ -252,6 +255,15 @@ lemma guarded_to_cur_domain:
   by (auto simp: invs_def valid_state_def valid_idle_def pred_tcb_at_def
                  obj_at_def ct_in_state_def guarded_pas_domain_def)
 
+lemma sts_ct_in_state:
+  "\<lbrace>\<lambda>s. t = cur_thread s \<and> P ts\<rbrace> set_thread_state t ts \<lbrace>\<lambda>rv. ct_in_state P\<rbrace>"
+  unfolding ct_in_state_def
+  apply (rule hoare_pre)
+   apply wps
+   apply (wpsimp wp: sts_st_tcb_at'')
+  apply clarsimp
+  done
+
 lemma handle_invocation_pas_refined:
   "\<lbrace>pas_refined aag and guarded_pas_domain aag and domain_sep_inv (pasMaySendIrqs aag) st'
                     and einvs and ct_active and schact_is_rct and is_subject aag \<circ> cur_thread\<rbrace>
@@ -259,25 +271,23 @@ lemma handle_invocation_pas_refined:
    \<lbrace>\<lambda>_. pas_refined aag\<rbrace>"
   apply (simp add: handle_invocation_def split_def)
   apply (cases blocking, simp)
-  by (((wp syscall_valid without_preemption_wp
-           handle_fault_pas_refined set_thread_state_pas_refined
-           set_thread_state_runnable_valid_sched
-           perform_invocation_pas_refined
-           hoare_vcg_conj_lift hoare_vcg_all_lift
-        | wpc
-        | rule hoare_drop_imps
-        | simp add: if_apply_def2 conj_comms split del: if_split
-               del: hoare_True_E_R)+),
-       ((wp lookup_extra_caps_auth lookup_extra_caps_authorised
-            decode_invocation_authorised
-            lookup_cap_and_slot_authorised
-            lookup_cap_and_slot_cur_auth
-            as_user_pas_refined
-            lookup_cap_and_slot_valid_fault3
-         | simp add: comp_def runnable_eq_active)+),
-       (auto intro: guarded_to_cur_domain
-              simp: ct_in_state_def st_tcb_at_def live_def
-             intro: if_live_then_nonz_capD)[1])+
+  (* slow ~30s *)
+  by ((wp syscall_valid without_preemption_wp handle_fault_pas_refined
+             set_thread_state_pas_refined set_thread_state_runnable_valid_sched
+             perform_invocation_pas_refined hoare_vcg_conj_lift hoare_vcg_all_lift
+             rfk_invs sts_st_tcb_at'' sts_ct_in_state
+       | strengthen invs_psp_aligned invs_vspace_objs invs_arch_state
+       | wpc
+       | rule hoare_drop_imps
+       | simp add: if_apply_def2 conj_comms split del: if_split
+              del: hoare_True_E_R)+,
+      (wp lookup_extra_caps_auth lookup_extra_caps_authorised decode_invocation_authorised
+          lookup_cap_and_slot_authorised lookup_cap_and_slot_cur_auth as_user_pas_refined
+          lookup_cap_and_slot_valid_fault3 hoare_vcg_const_imp_lift_R
+       | simp add: comp_def runnable_eq_active split del: if_split)+,
+       fastforce intro: guarded_to_cur_domain if_live_then_nonz_capD
+                  simp: ct_in_state_def st_tcb_at_def live_def)+
+
 
 lemma handle_invocation_respects:
   "\<lbrace>integrity aag X st and pas_refined aag and guarded_pas_domain aag
@@ -359,6 +369,7 @@ lemma handle_recv_integrity:
       apply (fastforce simp: aag_cap_auth_def cap_auth_conferred_def
                              cap_rights_to_auth_def valid_fault_def)
      apply wpsimp+
+  apply fastforce
   done
 
 lemma handle_reply_pas_refined[wp]:
@@ -546,7 +557,8 @@ interpretation handle_hypervisor_fault: Syscall_AC_wps "handle_hypervisor_fault 
   by simp
 
 lemma handle_interrupt_pas_refined:
-  "handle_interrupt irq \<lbrace>pas_refined aag\<rbrace>"
+  "\<lbrace>pas_refined aag and pspace_aligned and valid_vspace_objs and valid_arch_state\<rbrace>
+    handle_interrupt irq \<lbrace>\<lambda>_. pas_refined aag\<rbrace>"
   apply (simp add: handle_interrupt_def)
   apply (rule conjI; rule impI;rule hoare_pre)
   apply (wp send_signal_pas_refined get_cap_wp
@@ -645,7 +657,7 @@ lemma handle_event_pas_refined:
              hoare_vcg_conj_lift hoare_vcg_all_lift
           | wpc
           | rule hoare_drop_imps
-          | strengthen invs_vobjs_strgs
+          | strengthen invs_vobjs_strgs invs_psp_aligned invs_vspace_objs invs_arch_state
           | simp)+
   done
 
@@ -711,7 +723,9 @@ lemma activate_thread_integrity:
   done
 
 lemma activate_thread_pas_refined:
-  "activate_thread \<lbrace>pas_refined aag\<rbrace>"
+  "\<lbrace>pas_refined aag and pspace_aligned and valid_vspace_objs and valid_arch_state\<rbrace>
+   activate_thread
+   \<lbrace>\<lambda>_. pas_refined aag\<rbrace>"
   unfolding activate_thread_def get_thread_state_def thread_get_def
   apply (wpsimp wp: set_thread_state_pas_refined hoare_drop_imps)
   done
@@ -1164,8 +1178,9 @@ lemma call_kernel_pas_refined:
    \<lbrace>\<lambda>_. pas_refined aag\<rbrace>"
   apply (simp add: call_kernel_def )
   apply (wp activate_thread_pas_refined schedule_pas_refined handle_interrupt_pas_refined
-            do_machine_op_pas_refined dmo_wp alternative_wp select_wp)
-    apply (wpsimp wp: getActiveIRQ_inv)
+            do_machine_op_pas_refined dmo_wp alternative_wp select_wp hoare_drop_imps getActiveIRQ_inv
+         | simp add: if_fun_split
+         | strengthen invs_psp_aligned invs_vspace_objs invs_arch_state)+
    apply (wp he_invs handle_event_pas_refined)
   apply auto
   done
